
\subsection[SO*(2n)]{$\mathrm{SO}^*(2n) \sim D_n, n\geq 4$}

\subsubsection{Root system data}

\[\alpha_i = \epsilon_i - \epsilon_{i+1}, i<n, \alpha_n = \epsilon_{n-1} + \epsilon_n\]
\[\omega_i = \epsilon_1+\cdots \epsilon_i, i < n-1, \quad \omega_{n-1} = \frac{1}{2}(\epsilon_1 + \cdots \epsilon_{n-1}-\epsilon_n), \quad \omega_{n} = \frac{1}{2}(\epsilon_1 + \cdots \epsilon_{n-1}+\epsilon_n)\]
\begin{align*}
 \roots &= \{ \pm \epsilon_i \pm \epsilon_j | i\neq j, i,j = 1\ldots n \} \\
 \roots_c^+ &= \{ \epsilon_i-\epsilon_j | 1\leq i < j \leq  n\}\\
 \roots_n^+ &= \{ \epsilon_i + \epsilon_j | 1 \leq i <  j \leq n \}
\end{align*}
\[\beta = \epsilon_1+\epsilon_2,\quad \rho = (n-1,\ldots ,1,0),\quad \zeta = \frac{1}{2}(1,1,\ldots,1)\]
\inserttikzfigure{diagrams/dynkin_Dn_n.tikz}{Marked Dynkin diagram for $\mathrm{SO}^*(2n)$}

\begin{center}
\resizebox{\textwidth}{!}{
\begin{threeparttable}
\begin{tabular}{CCCCC}
  \text{Vertex } \lambda_a & \text{Weight } \mu_a &  Q(\lambda_a) = R(\lambda_a)& l(\lambda_a) \\ \hline
  \omega_2 - (2n-2)\omega_n & -(2n-2)\omega_n & \mathrm{SU}(1,1) &  1 \\
  \omega_p -2(n-p+l) \omega_n & \omega_{p-2l}-2(n-p+l)\omega_n & \mathrm{SO}^*(2p)\tnote{1} & 1\leq l \leq \floor{\frac{p}{2}} \\
  \omega_{n-1} - (1+2l)\omega_n & \omega_{n-1-2l} - 2(1+l)\omega_n &  \mathrm{SO}^*(2n-2) & 1\leq l \leq \floor{\frac{n-1}{2}} \\
  -(2l-2)\omega_n & \omega_{n-2l} - 2l\omega_n &  \mathrm{SO}^*(2n)  & 1\leq l \leq \floor{\frac{n}{2}} \\
  \omega_1 +\omega_{q+1} - (2n-q)\omega_n & \omega_q -(2n-q)\omega_n & \mathrm{SU}(1,q)\tnote{2} & 1\\
  \omega_1 +\omega_{n-1} - (n+1)\omega_n & \omega_{n-2} - (n+2)\omega_n &  \mathrm{SU}(1,n-2)  & 1 \\
  \omega_1 -(n-1)\omega_n & \omega_{n-1} - n\omega_n &  \mathrm{SU}(1,n-1)  & 1
\end{tabular}
\smallskip
\begin{tablenotes}
 \item [1] $3 \leq p \leq n-2$
 \item [2] $2 \leq q \leq n-3$
\end{tablenotes}\caption{Vertices and root systems for $\mathrm{SO}^*(2n)$, $n\geq 4$}\label{tbl:so_star}
\end{threeparttable}
}
\end{center}

Let $a=(Q,R,l)$, $Q=R$. Then for $R=\mathrm{SO}^*(2p)$, $3\leq p\leq n$
\[
 C_a = \{a_p\omega_p+\cdots + a_n\omega_n \,|\, a_n = -2a_p - \cdots -2a_{n-2} - a_{n-1}\}
\]
and for  $R=\mathrm{SU}(1,q)$, $1\leq q \leq n-1$
\[
 C_a = \{a_1\omega_1 + a_{q+1}\omega_{q+1} + \cdots + a_n\omega_n \,|\, a_n = -(a_1 + 2a_{q+1} + \cdots + 2a_{n-2} + a_{n-1})\}.
\]

\subsubsection{Nilpotent cohomology in detail}

Scalar products of positive noncompact roots with $\rho$ are
\[
 (\epsilon_i + \epsilon_j, \rho) = 2n - i -j.
\]

\begin{enumerate}
 \item $\lambda =  \omega_2 - (2n-2)\omega_n $\\
  \[
   (\epsilon_i + \epsilon_j,\lambda+\rho) = \begin{cases}
                                             1, &  i=1,j=2 \\
                                             2-j, & i=1, 2 < j \leq n\\
                                             1-j, & i=2, 2 < j \leq n \\
                                             2-i-j, & 2 < i < j
                                            \end{cases}
  \]
  \[
   \Psi^+_\lambda = \emptyset, \quad \roots^+_{n,\lambda} = \{ \epsilon_1 + \epsilon_2 \}
  \]
  
	Since the reduced pair is of rank 1, the whole cohomology is given in the table \ref{tbl:so_even}.

 \item $\lambda = \omega_p -2(n-p+l) \omega_n$, $3\leq p \leq n-2$, $1\leq l \leq \floor{\frac{p}{2}}$\\
  \[
   (\epsilon_i + \epsilon_j,\lambda+\rho) = \begin{cases}
                                             2(p-l+1)-i-j, & 1\leq i < j \leq p \\
                                             2(p-l)+1-i-j, & 1 \leq i \leq p < j \leq n\\
                                             2(p-l)-i-j, &  p <i < j \leq n
                                            \end{cases}
  \]
  \begin{align*}
   \Psi^+_\lambda & = \{ \epsilon_i + \epsilon_{2(p-l)+1-i} \,|\, \max\{1,1+2(p-l)-n\} \leq i < p-2l+1 \} \cup \\ &\qquad \{ \epsilon_i + \epsilon_{2(p-l)+2-i} \,|\, p-2l+2 \leq i < p-l+1 \}
  \end{align*}
  \begin{align*}
	M_\lambda &= \{1, \ldots,\max\{0,2(p-l)-n\}, p-2l+1, p-l+1  \} \\
    \roots^+_{n,\lambda} &= \{ \epsilon_i + \epsilon_j \,|\,  i,j \in M_\lambda \et i < j \}
  \end{align*}

  
 \item $\lambda = \omega_{n-1} - (1+2l)\omega_n  $, $  1\leq l \leq \floor{\frac{n-1}{2}}$  \\
  \[
   (\epsilon_i + \epsilon_j,\lambda+\rho) = \begin{cases}
                                             2(n-l)-i-j, & 1 \leq i<	j < n \\
                                             n-2l-1-i, & 1 \leq i< n = j
                                            \end{cases}
  \]
  \begin{enumerate}
   \item $n$ is odd and $l=\frac{n-1}{2}$\\
    \[
      \Psi^+_\lambda = \Big\{\epsilon_i + \epsilon_{n+1-i} \,\big|\, 1<i< \frac{n+1}{2} \Big\}
    \]
    \[
      \roots^+_{n,\lambda} = \left\{ \epsilon_1 + \epsilon_{\frac{n+1}{2}} \right\}
    \]
    
   \item $n$ even or $n$ odd and $l < \frac{n-1}{2}$\\
    \[
      \Psi^+_\lambda = \{\epsilon_i + \epsilon_{2(n-l)-i} \,|\, n-2l<i<n-l \} \cup \{ \epsilon_{n-2l-1} + \epsilon_n \}
    \]
    \[
      \roots^+_{n,\lambda} = \{ \epsilon_i + \epsilon_j \,|\, i < j \et i,j\in \{1,\ldots,n-2l-2,n-2l,n-l\} \}
    \]
  \end{enumerate}
  
 \item $\lambda = -(2l-2)\omega_n $, $ 1\leq l \leq \floor{\frac{n}{2}} $\\
 \[
  (\epsilon_i + \epsilon_j,\lambda+\rho) = 2(n-l+1)-i-j
 \]
 \[
  \Psi^+_\lambda = \{ \epsilon_i + \epsilon_{2(n-l+1)-i} \,|\, n + 2(1-l) \leq i \leq n-l  \} 
 \]
 \[
  \roots^+_{n,\lambda} =  \{ \epsilon_i + \epsilon_j \,|\, i < j \et i,j \in \{ 1,\ldots, n-2l+1,n-l+1 \} \}
 \]

 
 \item $\lambda =  \omega_1 +\omega_{q+1} - (2n-q)\omega_n$, $ 2\leq q \leq n-3$\\
  \[
   (\epsilon_i + \epsilon_j,\lambda+\rho) = \begin{cases}
                                             2+q-j, & i = 1, 2\leq j \leq q+1 \\
                                             1+q-j, & i = 1, q+1 < j \leq n \\
                                             2+q-i-j, & 2\leq i < j \leq q+1 \\ % here are the only singular roots
                                             1+q-i-j, & 2\leq i \leq q+1 < j \leq n \\
                                             q-i-j, &   q+1 < i < j \leq n \\
                                            \end{cases}
  \]
  \[
   \Psi^+_\lambda = \Big\{ \epsilon_i + \epsilon_{2+q-i} \,\big|\, 1 < i < \frac{q}{2}+1 \Big\}
  \]
  \[
   \roots^+_{n,\lambda} = \begin{cases}
                           \{ \epsilon_1 + \epsilon_{q+1}  \}, & q \text{ is odd}\\
                           \big\{ \epsilon_1 + \epsilon_{q+1}, \epsilon_1 + \epsilon_{\frac{q}{2}+1}   \big\}, & q \text{ is even}
                          \end{cases}
  \]
  
 \item $\lambda = \omega_1 +\omega_{n-1} - (n+1)\omega_n $\\
  \[
   (\epsilon_i + \epsilon_j,\lambda+\rho) = \begin{cases}
                                             n - j, & i = 1 < j < n \\
                                             -1, & i = 1, j=n\\
                                             n-i-j, & 1 < i < j < n\\
                                             -1-i, & 1 < i < n = j
                                            \end{cases}
  \]
  \[
   \Psi^+_\lambda = \Big\{ \epsilon_i + \epsilon_{n-i} \,\big|\, 1 < i < \frac{n}{2}\Big\}, \quad 
   \roots^+_{n,\lambda} = \begin{cases}
				\{\epsilon_1 + \epsilon_{n-1} \}, & n \text{ is odd} \\
				\{\epsilon_1 + \epsilon_{n-1}, \epsilon_1 + \epsilon_{\frac{n}{2}} \}, & n \text{ is even}
			  \end{cases}
  \]
  
 \item $\lambda = \omega_1 -(n-1)\omega_n $\\
 \[
  (\epsilon_i + \epsilon_j,\lambda+\rho) = \begin{cases}
                                            n+1-j, & i=1<j\leq n\\
                                            n+1-i-j, & 1<i<j\leq n
                                           \end{cases}
 \]
 \[
   \Psi^+_\lambda = \Big\{\epsilon_i + \epsilon_{n+1-i} \,\big|\, 1 < i < \frac{n+1}{2} \Big\}
 \]
 \[
   \roots^+_{n,\lambda} = \begin{cases}
				\{\epsilon_1 + \epsilon_n \}, & n \text{ is even} \\
				\{\epsilon_1 + \epsilon_n, \epsilon_1 + \epsilon_{\frac{n+1}{2}} \}, & n \text{ is odd}
			  \end{cases}
  \]
\end{enumerate}

\begin{figure}[H]
  \centering
  \input{diagrams/nroots_D5_5.tikz} 
	\input{diagrams/bruhat_D5_5.tikz} 
  \caption{Poset of noncompact roots and the BGG graph for $\mathrm{SO}^*(10)$}
\end{figure} 
